$\displaystyle - \dv{\gamma} \hat{f}(\gamma) = \mcu(2\pi i x f(x))$
\begin{proof}
    \begin{align*}
        - \dv{\gamma} \hat{f}(\gamma) &=  - \dv{\gamma}  \pars{ \intreal f(\gamma) e^{-2 \pi i \gamma x} \dd \gamma}\\
        &= \pars{ \intreal f(\gamma) - \dv{\gamma} e^{-2 \pi i \gamma x} \dd \gamma}\\
        &= -\pars{ \intreal f(\gamma) -2 \pi ix e^{-2 \pi i \gamma x} \dd \gamma}\\
        &=  2 \pi ix \pars{ \intreal f(\gamma) e^{-2 \pi i \gamma x}\dd \gamma}\\
        &= \mcu(2\pi i x f(\gamma))
    \end{align*}
\end{proof}