$\mcu(e^{-2 \pi i a x } f(x)) = \hat{f}(\gamma - a)$
\begin{proof}
    I changed the exponent sign, I believe it was wrong.
    \begin{align*}
        \hat{f}(\gamma - a) &= \hat{g}(\gamma)\\
        &= \intreal g(t) e^{-2\pi i x t} \dd t \\
        &= \intreal f(t-a)e^{-2\pi i x t} \dd t \\
        &=  \intreal f(u)e^{-2\pi i x (u+a)} \dd u \tag{$u=t-a,\; t = u+a$} \\
        &= e^{-2\pi i x a} \intreal f(u)e^{-2\pi i x u} \dd u \\
        &= e^{-2\pi i x a} \hat{f}(x)
    \end{align*}
\end{proof}