Find the Fourier Series of $f$.

\soln* Goal: $\displaystyle \widehat{f}(t) = \frac{a_0}{2} + \sumn{0} a_n \cosp{\nptl} + \sumn{1} b_n \sinp{\nptl}$. Here, since the period is length 6, $6 = 2L \implies L = 3$. 

\begin{align*}
    a_0 &= \frac{1}{L} \intll f(t) \dd t \\
    &= \frac{1}{3} \symint{3} f(t) \dd t \\
    &= \frac13 \pars{ \int_{-3}^0 -t \dd t + \int_{0}^3 t^2 \dd t}\\ 
    &= \frac13 \pars{ \brac{\frac{-t^2}{2}}_{-3}^{0} + \brac{\frac{t^3}{3}}_{0}^{3} }\\
    &= \frac13 \pars{0 + \frac92 + \frac{27}{3}-0}\\
    &= \frac92
\end{align*}

\newpage
For the odd series coefficients...
\begin{align*}
    a_n &= \over{L} \intll f(t) \cosp{\nptl} \dd t\\
    &= \over3 \symint{3} f(t) \cosp{\npto3} \dd t \\
    &= \frac13 \Bigg(
        \underbrace{
            \int_{-3}^0 -t \cosp{\npto3} \dd t
        }_{\ast}
        + \underbrace{
            \int_{0}^3 t^2 \cosp{\npto3} \dd t
        }_{\ast\ast}
    \Bigg)
\end{align*}

\begin{align*}
    * &= - \int_{-3}^0 t \cosp{\npto3} \dd t \\
      &= - \brac{
            \frac{3t}{n \pi} \sinp{\npto3} + \frac{9}{n^2 \pi^2} \cosp{\npto3}
        }_{t=-3}^{t=0} \tag{by MW-1}\\
      &= -\brac{
        \pars{
            0 + \frac{9}{n^2 \pi^2} \cosp{0}
          } - \pars{
            \frac{-9}{n \pi} \sinp{-\np} + \frac{9}{n^2 \pi^2} \cosp{-\np}
          }
      } \\
      &= -\brac{
        \frac{9}{n^2 \pi^2} - \pars{
            \frac{9}{n \pi} \sinp{\np} + \frac{9}{n^2 \pi^2} \cosp{\np}
          }
      }  \tag{\text{even and odd props}}\\
      &= -\brac{
        \frac{9}{n^2 \pi^2} -
            \frac{9}{n^2 \pi^2} \cosp{\np}
      }  \tag{$\sin{\np} = 0$}\\
      &=  \frac{9}{n^2 \pi^2} \pars{
        \cosp{\np} - 1
      }
\end{align*}


\begin{align*}
    ** &=  \int_{0}^3 t^2 \cosp{\npto3} \dd t\\
    &= \brac{
        \frac{3t^2}{n \pi} \sinp{\npto3} + \frac{18t}{n^2 \pi^2} \cosp{\npto3} - \frac{54}{n^3 \pi^3} \sinp{\npto3}
    }_{t=0}^{t=3} \tag{by MW-3}\\
    &= \pars{
        \frac{27}{n \pi} \sinp{\np} + \frac{54}{n^2 \pi^2} \cosp{\np} - \frac{54}{n^3 \pi^3} \sinp{\np}
    } \\ & \quad - \pars{
        \frac{0}{n \pi} \sinp{0} + \frac{0}{n^2 \pi^2} \cosp{0} - \frac{54}{n^3 \pi^3} \sinp{0}
    } \\
    &= \frac{54}{n^2 \pi^2} \cosp{\np} \tag{$\sin{\np} = 0$}
\end{align*}

Thus 
\begin{align*}
    a_n &= \frac13 \pars{ \ast + \ast \ast}\\
    &= \frac13 \pars{
        \frac{9}{n^2 \pi^2} \pars{
            1 - \cosp{\np}
          } + \frac{54}{n^2 \pi^2} \cosp{\np}
    } \\
    &= \frac{27\cosp{\np} - 3}{n^2 \pi^2}
\end{align*}

%%
%%
%%
%%
%%
%%
% B_n
%%
%%
%%
%%
%%
%%
Next for the odd series,
\begin{align*}
    b_n &= \frac{1}{L} \intll f(t) \sinp{\nptl} \dd t \\
    &= \frac13 \Bigg(
        -\underbrace{
            \int_{-3}^0 t \sinp{\npto3} \dd t
        }_{\ast}
        + \underbrace{
            \int_{0}^3 t^2 \sinp{\npto3} \dd t
        }_{\ast\ast}
    \Bigg)
\end{align*}

First, 
\begin{align*}
    \ast &= \int_{-3}^0 t \sinp{\npto3} \dd t \\
    &= \brac{ \frac{-3t}{n \pi} \cosp{\npto3} + \frac{9}{n^2 \pi^2} \sinp{\npto3}}_{t=-3}^{t=0} \tag{by MW-2}\\
    &= \pars{
        \frac{0}{n \pi} \cosp{\npto3} + \frac{9}{n^2 \pi^2} \sinp{0}
    } - \pars{
        \frac{9}{n \pi} \cosp{-\np} + \frac{9}{n^2 \pi^2} \sinp{-\np}
    } \\
    &= -\frac{9}{n \pi} \cosp{\np} \tag{by cosine evenness and $\sin \np = 0$}
\end{align*}

Then
\begin{align*}
    ** &=  \int_{0}^3 t^2 \sinp{\npto3} \dd t\\
    &= \brac{
        \onp{-3t^2} \cosp{\npto3} 
        + \onps{18t} \sinp{\npto3} + \onpc{54} \cosp{\npto3}
    }_{t=0}^{t=3} \tag{by MW-4}\\
    &= \pars{
        \onp{-27} \cosp{\np} + 0 +   \onpc{54} \cosp{\np}
    } - \pars{
        0 + 0 + \onpc{54} \cosp{0}
    } \\
    &=  \onp{-27} \cosp{\np} +  \onpc{54} \pars{ \cosp{\np} - 1}
\end{align*}

Thus 
\begin{align*}
    b_n &= \frac{1}{3} \pars{\ast\ast - \ast}\\
    &=  \onpc{54} \pars{ \cosp{\np} - 1} - \onp{18} \cosp{\np}
\end{align*}

Finally, substituting all of this into  $\displaystyle \widehat{f}(t) = \frac{a_0}{2} + \sumn{0} a_n \cosp{\nptl} + \sumn{1} b_n \sinp{\nptl}$ yields
\begin{align*}
    \widehat{f}(t) &= \frac{9}{4} + \sumn0
    \pars{
        \cosp{\nptl} \pars{
            \frac{27\cosp{\np} - 3}{n^2 \pi^2}
        }
    }  \\
    & \qquad + \sumn1 \pars{
        \sinp{\nptl} \pars{
            \onpc{54} \pars{ \cosp{\np} - 1} - \onp{18} \cosp{\np}
        }
    }
\end{align*}

\newpage